common/Events.v
@@ -2193,11 +2193,7 @@ Section VISIBLE.
              (ef: external_function) (ge: Senv.t) (m: mem) (args: list val) tr rv m' : Prop :=
     match ef with
     | EF_external cp name sg => False
-    | EF_builtin cp name sg | EF_runtime cp name sg =>
-                             match lookup_builtin_function name sg with
-                             | None => False
-                             | _ => True
-                             end
+    | EF_builtin cp name sg | EF_runtime cp name sg => False
     | EF_inline_asm cp txt sg clb => False
     | _ => (external_call ef ge args m tr rv m') /\ (tr <> E0)
     end.
